DynamoDbEncryption/dafny/DynamoDbEncryption/src/FilterExpr.dfy
@@ -1490,7 +1490,36 @@ module DynamoDBFilterExpr {
     values: Option<DDB.ExpressionAttributeValueMap>,
     names : Option<DDB.ExpressionAttributeNameMap>
   )
-    : Result<MaybeKeyId, Error>
+    : (ret : Result<MaybeKeyId, Error>)
+
+    //= specification/searchable-encryption/search-config.md#get-beacon-key-for-query
+    //= type=implication
+    //# If the [Beacon Key Source](#beacon-key-source) is a [Single Key Store](#single-key-store-initialization)
+    //# then `beacon key id` MUST be the configured [beacon key id](#beacon-key-id)
+    ensures !bv.keySource.keyLoc.MultiLoc? ==> ret == Success(DontUseKeyId)
+
+    ensures ret.Success? && bv.keySource.keyLoc.MultiLoc? && values.Some? ==>
+      && GetBeaconKeyIds(bv, keyExpr, values.value, names, []).Success?
+      && var soFar := GetBeaconKeyIds(bv, keyExpr, values.value, names, []).value;
+      && GetBeaconKeyIds(bv, filterExpr, values.value, names, soFar).Success?
+      && var final := GetBeaconKeyIds(bv, filterExpr, values.value, names, soFar).value;
+
+//= specification/searchable-encryption/search-config.md#get-beacon-key-for-query
+//= type=implication
+//# If this list of beacon key ids is empty get beacon key for query MUST
+//# return a flag indication this.
+      && (|final| == 0 ==> ret == Success(ShouldHaveKeyId))
+
+//= specification/searchable-encryption/search-config.md#get-beacon-key-for-query
+//= type=implication
+//# `beacon key id` MUST be this unique value.
+      && (|final| == 1 ==> ret == Success(KeyId(final[0])))
+
+//= specification/searchable-encryption/search-config.md#get-beacon-key-for-query
+//= type=implication
+//# If this list of beacon key ids has more than one unique beacon key id
+//# then get beacon key for query MUST fail.
+      && (|final| > 1 ==> ret.Failure?)
   {
     if !bv.keySource.keyLoc.MultiLoc? then
       Success(DontUseKeyId)
