DynamoDbEncryption/dafny/DynamoDbEncryption/Model/DynamoDbEncryption.smithy
@@ -90,6 +90,10 @@ structure DynamoDbTableEncryptionConfig {
     @required
     partitionKeyName: KeySchemaAttributeName,
     sortKeyName: KeySchemaAttributeName,
+
+    //= specification/searchable-encryption/search-config.md#overview
+    //= type=implication
+    //# The search config MUST be an optional part of the [item encryptor config](../dynamodb-encryption-client/ddb-item-encryptor.md).
     search: SearchConfig,
     
     @required
@@ -240,6 +244,12 @@ list ConstructorPartList {
   member: ConstructorPart
 }
 
+//= specification/searchable-encryption/virtual.md#virtual-field-initialization
+//= type=implication
+//# On initialization of a Virtual Field, the caller MUST provide:
+//#  * A name -- a string
+//#  * A list of [Virtual Parts](#virtual-part-initialization)
+
 structure VirtualField {
   @required
   name : String,
@@ -247,23 +257,51 @@ structure VirtualField {
   parts : VirtualPartList,
 }
 
+//= specification/searchable-encryption/virtual.md#virtual-part-initialization
+//= type=implication
+//# On initialization of a Virtual Part, the caller MUST provide:
+//# * A location -- a [Terminal Location](#terminal-location)
+
+//= specification/searchable-encryption/virtual.md#virtual-part-initialization
+//= type=implication
+//# On initialization of a Virtual Part, the caller MAY provide:
+//# * A list of [Virtual Transforms](#virtual-transform-initialization)
+
 structure VirtualPart {
   @required
   loc : TerminalLocation,
   trans : VirtualTransformList,
 }
 
+//= specification/searchable-encryption/virtual.md#upper-transform-initialization
+//= type=implication
+//# On initialization of an Upper Transform, the caller MUST NOT provide any further information
+
 // Convert ASCII characters to upper case
 structure Upper {}
 
+//= specification/searchable-encryption/virtual.md#lower-transform-initialization
+//= type=implication
+//# On initialization of a Lower Transform, the caller MUST NOT provide any further information
+
 // Convert ASCII characters to lower case
 structure Lower {}
+
+//= specification/searchable-encryption/virtual.md#insert-transform-initialization
+//= type=implication
+//# On initialization of an Insert Transform, the caller MUST provide:
+//# * a literal string
 
 // Append this literal string
 structure Insert {
   @required
   literal : String
 }
+
+//= specification/searchable-encryption/virtual.md#getprefix-transform-initialization
+//= type=implication
+//# On initialization of a GetPrefix Transform, the caller MUST provide:
+//#  * length : an integer
 
 // return the first part of the string
 // Positive length : return that many characters from the front
@@ -274,6 +312,11 @@ structure GetPrefix {
   length : Integer
 }
 
+//= specification/searchable-encryption/virtual.md#getsuffix-transform-initialization
+//= type=implication
+//# On initialization of a GetSuffix Transform, the caller MUST provide:
+//# * length : an integer
+
 // return the last part of the string
 // Positive length : return that many characters from the end
 // Negative length : exclude -length characters from the front
@@ -282,6 +325,12 @@ structure GetSuffix {
   @required
   length : Integer
 }
+
+//= specification/searchable-encryption/virtual.md#getsubstring-transform-initialization
+//= type=implication
+//# On initialization of a GetSubstring Transform, the caller MUST provide:
+//#  * low : an integer [position](#position-definition)
+//#  * high : an integer [position](#position-definition)
 
 // return range of characters, 0-based counting
 // low is inclusive, high is exclusive
@@ -296,6 +345,12 @@ structure GetSubstring {
   high : Integer,
 }
 
+//= specification/searchable-encryption/virtual.md#getsegment-transform-initialization
+//= type=implication
+//# On initialization of a GetSegment Transform, the caller MUST provide:
+//#  * split : an character
+//#  * index : an integer [position](#position-definition)
+
 // split string on character, then return one piece.
 // 'index' has the same semantics as 'low' in GetSubstring
 structure GetSegment {
@@ -305,7 +360,14 @@ structure GetSegment {
   index : Integer
 }
 
-// split string on character, then return range of pieces.
+//= specification/searchable-encryption/virtual.md#getsegments-transform-initialization
+//= type=implication
+//# On initialization of a GetSegments Transform, the caller MUST provide:
+//#  * split : an character
+//#  * low : an integer [position](#position-definition)
+//#  * high : an integer [position](#position-definition)
+
+//# split string on character, then return range of pieces.
 // 'low' and 'high' have the same semantics as GetSubstring
 structure GetSegments {
   @required
@@ -315,6 +377,18 @@ structure GetSegments {
   @required
   high : Integer,
 }
+
+//= specification/searchable-encryption/virtual.md#virtual-transform-initialization
+//= type=implication
+//# On initialization of a Virtual Transform, the caller MUST provide exactly one of
+//#  * an [Upper](#upper-transform-initialization) transform
+//#  * a [Lower](#lower-transform-initialization) transform
+//#  * an [Insert](#insert-transform-initialization) transform
+//#  * a [GetPrefix](#getprefix-transform-initialization) transform
+//#  * a [GetSuffix](#getsuffix-transform-initialization) transform
+//#  * a [GetSubstring](#getsubstring-transform-initialization) transform
+//#  * a [GetSegment](#getsegment-transform-initialization) transform
+//#  * a [GetSegments](#getsegments-transform-initialization) transform
 
 union VirtualTransform {
   upper: Upper,
@@ -327,12 +401,29 @@ union VirtualTransform {
   segments : GetSegments
 }
 
+//= specification/searchable-encryption/beacons.md#sensitive-part-initialization
+//= type=implication
+//# On initialization of a [sensitive part](#sensitive-part-initialization), the caller MUST provide:
+//#  * A name -- a string, the name of a standard beacon
+//#  * A prefix -- a string
+
 structure SensitivePart {
   @required
   name : String,
   @required
   prefix : Prefix
 }
+
+//= specification/searchable-encryption/beacons.md#non-sensitive-part-initialization
+//= type=implication
+//# On initialization of a [non-sensitive part](#non-sensitive-part-initialization), the caller MUST provide:
+//#  * A name -- a string
+//#  * A prefix -- a string
+
+//= specification/searchable-encryption/beacons.md#non-sensitive-part-initialization
+//= type=implication
+//# On initialization of a [non-sensitive parts](#non-sensitive-part-initialization), the caller MAY provide:
+//# * A [terminal location](virtual.md#terminal-location) -- a string
 
 structure NonSensitivePart {
   @required
@@ -342,10 +433,21 @@ structure NonSensitivePart {
   loc : TerminalLocation
 }
 
+//= specification/searchable-encryption/beacons.md#constructor-initialization
+//= type=implication
+//# On initialization of a constructor, the caller MUST provide:
+//# * A non-empty list of [Constructor parts](#constructor-part-initialization)
+
 structure Constructor {
   @required
   parts : ConstructorPartList
 }
+
+//= specification/searchable-encryption/beacons.md#constructor-part-initialization
+//= type=implication
+//# On initialization of a constructor part, the caller MUST provide:
+//#  * A name -- a string
+//#  * A required flag -- a boolean
 
 structure ConstructorPart {
   @required
@@ -354,6 +456,17 @@ structure ConstructorPart {
   required : Boolean,
 }
 
+//= specification/searchable-encryption/beacons.md#standard-beacon-initialization
+//= type=implication
+//# On initialization of a Standard Beacon, the caller MUST provide:
+//#  * A name -- a string
+//#  * A `length` -- a [beacon length](#beacon-length)
+
+//= specification/searchable-encryption/beacons.md#standard-beacon-initialization
+//= type=implication
+//# On initialization of a Standard Beacon, the caller MAY provide:
+//# * a [terminal location](virtual.md#terminal-location) -- a string
+
 structure StandardBeacon {
   @required
   name : String,
@@ -361,6 +474,19 @@ structure StandardBeacon {
   length : BeaconBitLength,
   loc : TerminalLocation
 }
+
+//= specification/searchable-encryption/beacons.md#compound-beacon-initialization
+//= type=implication
+//# On initialization of a Compound Beacon, the caller MUST provide:
+//#  * A name -- a string
+//#  * A split character -- a character
+
+//= specification/searchable-encryption/beacons.md#compound-beacon-initialization
+//= type=implication
+//# On initialization of a Compound Beacon, the caller MAY provide:
+//#  * A list of [sensitive parts](#sensitive-part-initialization)
+//#  * A list of [non-sensitive parts](#non-sensitive-part-initialization)
+//#  * A list of constructors
 
 structure CompoundBeacon {
   @required
@@ -375,12 +501,25 @@ structure CompoundBeacon {
 @aws.polymorph#reference(service: aws.cryptography.keyStore#KeyStore)
 structure KeyStoreReference {}
 
+//= specification/searchable-encryption/search-config.md#single-key-store-initialization
+//= type=implication
+//# On initialization of a Single Key Store, the caller MUST provide:
+//#  - [Beacon Key Id](#beacon-key-id)
+//#  - [cacheTTL](#cachettl)
+
 structure SingleKeyStore {
   @required
   keyId : String,
   @required
   cacheTTL: Integer,
 }
+
+//= specification/searchable-encryption/search-config.md#multi-key-store-initialization
+//= type=implication
+//# On initialization of a Multi Key Store, the caller MUST provide:
+//#  - [Beacon Key Field Name](#beacon-key-field-name)
+//#  - [cacheTTL](#cachettl)
+//#  - [max cache size](#max-cache-size)
 
 structure MultiKeyStore {
   @required
@@ -391,10 +530,30 @@ structure MultiKeyStore {
   maxCacheSize: Integer
 }
 
+//= specification/searchable-encryption/search-config.md#beacon-key-source
+//= type=implication
+//# On initialization of a Beacon Key Source, the caller MUST provide exactly one of
+//#  * a [Single Key Store](#single-key-store-initialization)
+//#  * a [Multi Key Store](#multi-key-store-initialization)
+
 union BeaconKeySource {
   single : SingleKeyStore,
   multi : MultiKeyStore
 }
+
+//= specification/searchable-encryption/search-config.md#beacon-version-initialization
+//= type=implication
+//# On initialization of a Beacon Version, the caller MUST provide:
+//#  - A [version number](#version number)
+//#  - A [Beacon Key Source](#beacon-key-source)
+//#  - A [Keystore](#keystore)
+//#  - A list of [standard beacons](beacons.md#standard-beacon-initialization)
+
+//= specification/searchable-encryption/search-config.md#beacon-version-initialization
+//= type=implication
+//# On initialization of the Beacon Version, the caller MAY provide:
+//#  - A list of [compound beacons](beacons.md#compound-beacon-initialization)
+//#  - A list of [virtual fields](virtual.md#virtual-field-initialization)
 
 structure BeaconVersion {
   @required
@@ -405,9 +564,16 @@ structure BeaconVersion {
   keySource: BeaconKeySource,
   @required
   standardBeacons : StandardBeaconList,
+
   compoundBeacons : CompoundBeaconList,
   virtualFields : VirtualFieldList,
 }
+
+//= specification/searchable-encryption/search-config.md#initialization
+//= type=implication
+//# On initialization of the Search Config, the caller MUST provide:
+//#  - A list of [beacon versions](#beacon-version-initialization)
+//#  - The [version number](#version-number) of the [beacon versions](#beacon-version) to be used for writing.
 
 structure SearchConfig {
   @required
